Lean 4.15

Semantics/Imp/Aexp.lean
@@ -13,17 +13,13 @@ private inductive BigStep: Aexp × State → Int → Prop
   | mul (ha: BigStep (a, s) x) (ha': BigStep (a', s) y):
     BigStep (a * a', s) (x * y)
 
-infix:10 " ==> " => BigStep
+infix:100 " ==>a " => BigStep
 
 private instance equiv: Setoid Aexp where
-  r a a' := ∀{s n}, ((a, s) ==> n) ↔ ((a', s) ==> n)
-  iseqv := {
-    refl := fun _ => Iff.rfl
-    symm := (Iff.symm .)
-    trans := (Iff.trans . .)
-  }
+  r a a' := ∀{s n}, (a, s) ==>a n ↔ (a', s) ==>a n
+  iseqv := ⟨fun _ => Iff.rfl, (Iff.symm .), (Iff.trans . .)⟩
 
-private example: ((var "x" + 5) + (9 - 7), s0) ==> 7 :=
+private example: (var "x" + 5 + (9 - 7), s0) ==>a 7 :=
   .add (.add .var .val) (.sub .val .val)
 
 end BigStep
@@ -40,43 +36,35 @@ instance: CoeFun Aexp (fun _a => State → Int) := ⟨eval⟩
 
 instance reduce.equiv: Setoid Aexp where
   r a a' := ∀{s}, a s = a' s
-  iseqv := {
-    refl := fun _ => rfl
-    symm := (Eq.symm .)
-    trans := (Eq.trans . .)
-  }
+  iseqv := ⟨fun _ => rfl, (Eq.symm .), (Eq.trans . .)⟩
 
-#eval (var "x" + 5) + (9 - 7) $ s0 -- 7
+#eval var "x" + 5 + (9 - 7) $ s0 -- 7
 
 section Equivalence
 
 -- relational definition is equal to recursive
-private theorem reduce.from_natural
-  (hBigStep: conf ==> n): conf.1 conf.2 = n :=
-  by induction hBigStep with
+private theorem reduce.from_natural (h: conf ==>a n): conf.1 conf.2 = n :=
+  by induction h with
   | add _ _ iha iha' => exact iha ▸ iha' ▸ rfl
   | sub _ _ iha iha' => exact iha ▸ iha' ▸ rfl
   | mul _ _ iha iha' => exact iha ▸ iha' ▸ rfl
   | _ => rfl
 
-private theorem BigStep.from_reduce
-  (hred: a s = n): (a, s) ==> n :=
+private theorem BigStep.from_reduce (h: a s = n): (a, s) ==>a n :=
   by induction a generalizing n with
-  | val a => exact hred ▸ .val
-  | var a => exact hred ▸ .var
+  | val a => exact h ▸ .val
+  | var a => exact h ▸ .var
   | add a a' iha iha' =>
-    exact hred ▸ (iha rfl).add (iha' rfl)
+    exact h ▸ (iha rfl).add (iha' rfl)
   | sub a a' iha iha' =>
-    exact hred ▸ (iha rfl).sub (iha' rfl)
+    exact h ▸ (iha rfl).sub (iha' rfl)
   | mul a a' iha iha' =>
-    exact hred ▸ (iha rfl).mul (iha' rfl)
+    exact h ▸ (iha rfl).mul (iha' rfl)
 
-private theorem BigStep_eq_reduce:
-  ((a, s) ==> n) ↔ (a s = n) :=
+private theorem BigStep_eq_reduce: (a, s) ==>a n ↔ a s = n :=
   ⟨reduce.from_natural, BigStep.from_reduce⟩
 
-private theorem BigStep_eq_reduce':
-  (a, s) ==> a s :=
+private theorem BigStep_eq_reduce': (a, s) ==>a a s :=
   BigStep.from_reduce rfl
 
 private theorem BigStep_eq_eq_reduce_eq:
