Semantics/Imp/SmallStep.lean
@@ -4,24 +4,24 @@ import Semantics.ReflTransRel
 namespace Com
 
 inductive SmallStep: Com × State → Com × State → Prop where
-  | ass: SmallStep (ass v a, s) ({}, s[v ← a s])
-  | skipCat: SmallStep ({}++c, s) (c, s)
+  | ass: SmallStep (ass v a, s) (∅, s[v ← a s])
+  | skipCat: SmallStep (∅++c, s) (c, s)
   | cat (hstep: SmallStep (c, s) (c', s')):
     SmallStep (c++c'', s) (c'++c'', s')
   | ifElse: SmallStep (ifElse b c c', s) (cond (b s) c c', s)
   | whileLoop:
-    SmallStep (whileLoop b c, s) (cond (b s) (c++whileLoop b c) {}, s)
+    SmallStep (whileLoop b c, s) (cond (b s) (c++whileLoop b c) ∅, s)
 
-infixl:10 " ~> " => SmallStep
+infixl:100 " ~> " => SmallStep
 
 namespace SmallStep
 
 private example: ([|x = 1; while x <= 2 {x = x + 1}|], s0) ~>
   ([|skip; while x <= 2 {x = x + 1}|], s0["x" ← 1]) := cat ass
 
-theorem cat_eq: ((c++c'', s) ~> conf)
-  ↔ ((∃c' s', ((c, s) ~> (c', s')) ∧ conf = (c'++c'', s'))
-    ∨ (c = {} ∧ conf = (c'', s))) := {
+theorem cat_eq: (c++c'', s) ~> x
+  ↔ ((∃c' s', (c, s) ~> (c', s') ∧ x = (c'++c'', s'))
+    ∨ (c = ∅ ∧ x = (c'', s))) := {
     mp := fun hmp => match hmp with
       | skipCat => .inr ⟨rfl, rfl⟩
       | cat h => .inl ⟨_, _, h, rfl⟩,
@@ -30,27 +30,27 @@ theorem cat_eq: ((c++c'', s) ~> conf)
       | .inr ⟨hl, hr⟩ => hl ▸ hr ▸ skipCat
   }
 
-theorem cond_eq: ((.ifElse b c c', s) ~> conf)
-  ↔ (b s ∧ conf = (c, s) ∨ b s = false ∧ conf = (c', s)) := {
+theorem cond_eq: (.ifElse b c c', s) ~> x
+  ↔ (b s ∧ x = (c, s) ∨ b s = false ∧ x = (c', s)) := {
     mp := fun hmp => match hb: b s with
       | false => match hmp with | ifElse => .inr ⟨rfl, hb ▸ rfl⟩
       | true => match hmp with | ifElse => .inl ⟨rfl, hb ▸ rfl⟩,
     mpr := fun hmpr =>
-      have hss: conf = (cond (b s) c c', s) := match hb: b s with
+      have hss: x = (cond (b s) c c', s) := match hb: b s with
         | true => match hb ▸ hmpr with | .inl ⟨_, hr⟩ => hr
         | false => match hb ▸ hmpr with | .inr ⟨_, hr⟩ => hr
       hss ▸ ifElse
   }
 
-theorem cond_false (hb: b s = false): ((.ifElse b c c', s) ~> conf)
-  ↔ (conf = (c', s)) := by
+theorem cond_false (hb: b s = false): (.ifElse b c c', s) ~> x ↔ x = (c', s) :=
+  by
   rw [cond_eq, hb]
   exact ⟨fun (.inr ⟨rfl, h⟩) => h, (.inr ⟨rfl, .⟩)⟩
 
-infixl:10 " ~>* " => ReflTrans SmallStep
+infixl:100 " ~>* " => ReflTrans SmallStep
 
 private example: ([|x = 1; while x <= 1 {x = x + 1}|], s0) ~>*
-    ({}, s0["x" ← 1]["x" ← 2]) := by
+    (∅, s0["x" ← 1]["x" ← 2]) := by
   apply ReflTrans.head (cat ass) (ReflTrans.head skipCat _)
   apply ReflTrans.head whileLoop
   have hs : s0["x" ← Aexp.eval 1 s0] = s0["x" ← 1] := rfl
@@ -66,15 +66,15 @@ private example: ([|x = 1; while x <= 1 {x = x + 1}|], s0) ~>*
   rw [hs, hcond]
   apply ReflTrans.refl
 
-theorem star.cat_skip_cat (hc: (c, s) ~>* ({}, s')):
-  (c++c', s) ~>* ({}++c', s') :=
+theorem star.cat_skip_cat (hc: (c, s) ~>* (∅, s')):
+  (c++c', s) ~>* (∅++c', s') :=
   .lift (fun (c, s) => (c++c', s)) (cat .) hc
 
-theorem star.cat (hc: (c, s) ~>* ({}, s')) (hc': (c', s') ~>* ({}, s'')):
-  (c++c', s) ~>* ({}, s'') :=
+theorem star.cat (hc: (c, s) ~>* (∅, s')) (hc': (c', s') ~>* (∅, s'')):
+  (c++c', s) ~>* (∅, s'') :=
   .trans (cat_skip_cat hc) $ .trans (.single skipCat) hc'
 
-theorem star.cat_no_influence (hc: (c, s) ~>* ({}, s)):
+theorem star.cat_no_influence (hc: (c, s) ~>* (∅, s)):
   (c++c', s) ~>* (c', s) :=
   .trans (cat_skip_cat hc) $ .single skipCat
 
