Semantics/Imp/Equivalence.lean
@@ -4,9 +4,9 @@ import Semantics.Imp.Denotational
 
 namespace Com
 
-theorem SmallStep.from_natural {conf: Com × State}
-  (hconf: conf ==> s'): conf ~>* (skip, s') := by
-  induction hconf with
+theorem SmallStep.from_natural {x: Com × State}
+  (hx: x ==> s'): x ~>* (∅, s') := by
+  induction hx with
   | skip => exact .refl
   | ass => exact .single ass
   | cat _ _ _ ihcatl ihcatr => exact star.cat ihcatl ihcatr
@@ -18,28 +18,28 @@ theorem SmallStep.from_natural {conf: Com × State}
     exact .head whileLoop (hcond ▸ .refl)
 
 theorem BigStep.from_structural_step
-  (hconf: conf ~> conf') (hconf': conf' ==> s'): conf ==> s' := by
-  induction hconf generalizing s' with
-  | ass => exact (skip_eq.mp hconf') ▸ ass
-  | skipCat => exact cat _ skip hconf'
-  | cat _ ih => match hconf' with
+  (hx: x ~> x') (hx': x' ==> s'): x ==> s' := by
+  induction hx generalizing s' with
+  | ass => exact (skip_eq.mp hx') ▸ ass
+  | skipCat => exact cat _ skip hx'
+  | cat _ ih => match hx' with
     | cat s' hcatl hccatr => exact cat s' (ih hcatl) hccatr
-  | ifElse => rw [if_eq']; exact hconf'
-  | whileLoop => rw [loop_unfold, if_eq']; exact hconf'
+  | ifElse => rw [if_eq']; exact hx'
+  | whileLoop => rw [loop_unfold, if_eq']; exact hx'
 
 theorem BigStep.from_structural
-  (hconf: conf ~>* (.skip, s')): conf ==> s' := by
-  induction hconf using ReflTrans.head_induction_on with
+  (hx: x ~>* (∅, s')): x ==> s' := by
+  induction hx using ReflTrans.head_induction_on with
   | refl => exact skip
   | head hsingle _ hs' => exact from_structural_step hsingle hs'
 
 theorem structural_eq_natural:
-  ((c, s) ~>* (skip, s')) ↔ ((c, s) ==> s') :=
+  ((c, s) ~>* (∅, s')) ↔ ((c, s) ==> s') :=
   ⟨BigStep.from_structural, SmallStep.from_natural⟩
 
-theorem denote.from_natural {conf: Com × State}
-  (hconf: conf ==> s''): (conf.2, s'') ∈ [[conf.1]] := by
-  induction hconf with
+theorem denote.from_natural {x: Com × State}
+  (hx: x ==> s''): (x.2, s'') ∈ ⟦x.1⟧ := by
+  induction hx with
   | skip => exact rfl
   | ass  => exact rfl
   | cat s' _ _ ihcatl ihcatr => exact ⟨s', ihcatl, ihcatr⟩
@@ -53,7 +53,7 @@ theorem denote.from_natural {conf: Com × State}
     exact Denotational.while_unfold ▸
       .inr ⟨denote.eq_1 ▸ rfl, (absurd . (Bool.not_eq_true _ ▸ hcond))⟩
 
-theorem BigStep.from_denote (hmem: (s, s'') ∈ [[c]]): (c, s) ==> s'' := by
+theorem BigStep.from_denote (hmem: (s, s'') ∈ ⟦c⟧): (c, s) ==> s'' := by
   revert hmem
   induction c generalizing s s'' with
   | skip => exact (SRel.mem_id.mp . ▸ skip)
@@ -67,7 +67,7 @@ theorem BigStep.from_denote (hmem: (s, s'') ∈ [[c]]): (c, s) ==> s'' := by
     | .inr ⟨hstep, hcond⟩ =>
       exact ifFalse (Bool.not_eq_true _ ▸ hcond) (ih2 hstep)
   | whileLoop b c ih =>
-    have h: [[whileLoop b c]] ≤ {(s, s'') | (whileLoop b c, s) ==> s''} :=
+    have h: ⟦whileLoop b c⟧ ≤ {(s, s'') | (whileLoop b c, s) ==> s''} :=
       OrderHom.lfp_le fun (_, _) hmp =>
         match hmp with
         | .inl ⟨⟨s', hstep, hrest⟩, hcond⟩ =>
@@ -77,10 +77,10 @@ theorem BigStep.from_denote (hmem: (s, s'') ∈ [[c]]): (c, s) ==> s'' := by
 
     apply h
 
-theorem natural_eq_denote: ((s, s') ∈ [[c]]) ↔ ((c, s) ==> s') :=
+theorem natural_eq_denote: ((s, s') ∈ ⟦c⟧) ↔ ((c, s) ==> s') :=
   ⟨BigStep.from_denote, denote.from_natural⟩
 
-theorem structural_eq_denote: ((c, s) ~>* (skip, s')) = ((s, s') ∈ [[c]]) :=
+theorem structural_eq_denote: ((c, s) ~>* (∅, s')) = ((s, s') ∈ ⟦c⟧) :=
   by rw [structural_eq_natural, natural_eq_denote]
 
 end Com
